proof poly1305 cleanup

proof/crypto_onetimeauth/poly1305/Poly1305_Spec.ec
@@ -1,6 +1,25 @@
-require import List Jasmin_model Int IntExtra IntDiv CoreMap Real.
+require import List Int IntExtra IntDiv CoreMap Real.
+from Jasmin require import JModel.
 require import Zp.
 import Zp.
+
+
+(* ?move elsewhere? *)
+lemma loadW128_storeW128_eq mem ptr a : loadW128 (storeW128 mem ptr a) ptr = a.
+proof.
+rewrite /loadW128 storeW128E -{2}(W16u8.unpack8K a); congr.
+apply W16u8.Pack.packP => i hi. 
+by rewrite initE hi /= get_storesE /= get_unpack8 1:// /#.
+qed.
+
+lemma storeW128_inj_w m p w1 w2: storeW128 m p w1 = storeW128 m p w2 => w1=w2.
+proof.
+rewrite -{2}(loadW128_storeW128_eq m p w1) => ->.
+by rewrite loadW128_storeW128_eq.
+qed.
+
+
+
 
 (****************************************************************)
 (************ HACL* - Specification   **********************)
@@ -125,12 +144,16 @@ lemma load16u8vs128 (mem : global_mem_t) (ptr : W64.t) :
             (fun i => if i < 16 
                       then mem.[to_uint ptr + i] 
                       else W8.zero)).
+proof.
 rewrite /loadW128.
-have ? : forall i, 0<=i<16 => (mem.[to_uint ptr + i])= (if i < 16 then mem.[to_uint ptr + i] else W8.zero). smt(). 
-move : (W16u8.Pack.init_ext 
-            (fun (i : int) => mem.[to_uint ptr + i])
-            (fun (i : int) => if i < 16 then mem.[to_uint ptr + i] else W8.zero)).
-smt.
+have ? : forall i, 0<=i<16 =>
+           mem.[to_uint ptr + i]
+           = if i < 16 then mem.[to_uint ptr + i] else W8.zero
+ by smt(). 
+move: (W16u8.Pack.init_ext 
+        (fun (i : int) => mem.[to_uint ptr + i])
+        (fun (i : int) => if i < 16 then mem.[to_uint ptr + i] else W8.zero)).
+smt().
 qed.
 
 lemma full_block (mem : global_mem_t) (ptr : W64.t):
@@ -183,8 +206,8 @@ module Mspec = {
 }.
 
 (* Bounded memory assumption (established by the safety analysis) *)
-abbrev good_ptr (ptr: W64.t) len =
- to_uint ptr + len < W64.modulus.
+abbrev good_ptr (ptr: W64.t) len = to_uint ptr + len < W64.modulus.
+
 op inv_ptr (k in_0 len out: W64.t) =
  good_ptr k 32 /\ good_ptr in_0 (to_uint len) /\ good_ptr out 16.
 
@@ -192,17 +215,16 @@ op inv_ptr (k in_0 len out: W64.t) =
                             represented in memory *)
 op poly1305_pre (r : zp) (s : int) (m : Zp_msg)
                 (mem : global_mem_t) (inn, inl, kk : W64.t)  = 
-      (size m = if  W64.to_uint inl %% 16 = 0 
+ (size m = if  W64.to_uint inl %% 16 = 0 
            then to_uint inl %/ 16
            else to_uint inl %/ 16 + 1) /\
-       m = mkseq (fun i => 
-            let offset = W64.of_int (i * 16) in
-               if i < size m - 1
-               then load_block mem (inn + offset)
-               else load_lblock mem (inl - offset) (inn + offset))
-                     (size m) /\
-        r = load_clamp mem kk /\
-        s = to_uint (loadW128 mem (to_uint (kk + W64.of_int 16))).
+  m = mkseq (fun i => 
+             let offset = W64.of_int (i * 16) in
+             if i < size m - 1
+             then load_block mem (inn + offset)
+             else load_lblock mem (inl - offset) (inn + offset)) (size m) /\
+  r = load_clamp mem kk /\
+  s = to_uint (loadW128 mem (to_uint (kk + W64.of_int 16))).
 
 (* Relational postcondition: output of specification is
                              stored in memory *)
@@ -210,23 +232,17 @@ op poly1305_post mem_pre mem_post outt rr ss mm =
   mem_post = storeW128 mem_pre (W64.to_uint outt)
        (W128.of_int (poly1305_ref rr ss mm)).
 
-lemma loadW128_storeW128_eq mem ptr a : loadW128 (storeW128 mem ptr a) ptr = a.
-proof.
-  rewrite /loadW128 storeW128E.
-  rewrite -{2}(W16u8.unpack8K a);congr.
-  apply W16u8.Pack.packP => i hi. 
-  rewrite initE hi /= get_storesE /= get_unpack8 1:// /#.
-qed.
+
 
 equiv spec_eq mem rr ss mm outt inn inl kk :
-   Poly1305_RefWhile.poly1305 ~ Mspec.poly1305 : 
+ Poly1305_RefWhile.poly1305 ~ Mspec.poly1305 : 
       Glob.mem{2} = mem /\
       r{1} = rr /\ s{1} = ss /\ m{1} = mm /\
       out{2} = outt /\ in_0{2} = inn /\ inlen{2} = inl /\ k{2} = kk /\
-      poly1305_pre rr ss mm mem inn inl kk ==>
-        res{1} = poly1305_ref rr ss mm <=>
-          poly1305_post mem Glob.mem{2} outt rr ss mm.
-            
+      poly1305_pre rr ss mm mem inn inl kk
+    ==>
+      res{1} = poly1305_ref rr ss mm
+      <=> poly1305_post mem Glob.mem{2} outt rr ss mm.
 proof.
 proc.
 seq 3 3 : (#{~in_0{2}=inn}pre /\ 
@@ -235,128 +251,110 @@ seq 3 3 : (#{~in_0{2}=inn}pre /\
           0 <= i{1} /\
            ={h,r} /\ n{1} = size m{1} /\ i{1} <= n{1} /\ 
           to_uint inlen0{2} = to_uint inlen{2} - 16 * i{1} /\ 
-          in_0{2} = inn + W64.of_int (16 * i{1}));
-            first by 
-             auto => />;move => &1 &2 [/ # *];progress;[1: by smt(size_ge0)| 2..: by smt ].
+          in_0{2} = inn + W64.of_int (16 * i{1})).
+ auto => />;move => &1 &2 [/ # *]; progress; smt(size_ge0). 
 (* Iterations where while loops are always synched *)
 splitwhile {1} 1 : (i < n - 1).
 splitwhile {2} 1 : (16 < to_uint inlen0).
 seq 1 1 : (#{/~0 < n{1} => i{1} <= n{1} - 1}pre /\ 
            (0 < n{1} => n{1} - 1 <= i{1})).
-while (#pre).
-auto => />;move => &1 &2 [/ # *].
-progress.
-by smt().
-by smt().
-by smt().
-rewrite H0 /mkseq onth_nth_map; 
-    rewrite (nth_map witness);
-      first by rewrite size_map size_iota /max;smt().
-    rewrite (nth_map witness);
-      first by rewrite size_iota /max;smt().
-    auto => />.
-    by rewrite nth_iota => /#.
-by smt().
-by smt.
-by smt.
-by smt.
-by smt.
-by smt.
-by smt.
-auto => />;move => &1 &2 [/ # *].
-progress.
-by smt. by smt. by smt. by smt. by smt.
-
+ while (#pre).
+  auto => />;move => &1 &2 [/ # *].
+  move: H8; rewrite !uleE; progress;
+  [ 1..3,5,7,10: smt()
+  | 4: rewrite H0 /mkseq onth_nth_map (nth_map witness);
+       [ rewrite size_map size_iota /max /#
+       | rewrite /= (nth_map witness) ?size_iota /max /= 1:/#
+                 nth_iota 1:/# /= H7 /# ]
+  | 6,8,9: by rewrite to_uintB ?uleE // /#
+  | 11: move: H11; rewrite to_uintB ?uleE // /#
+  ].
+ auto => />; rewrite !uleE; move => &1 &2 [/ # *]; progress; smt().
 seq 1 2 : (#{/~n{1}}{~i{1}}pre); last first.       
-  wp;skip;progress. smt. 
-  move :  H H0.
-  rewrite /poly1305_pre /poly1305_post /poly1305_ref => //= *. smt.
-
+ wp; skip; progress; first smt().
+ move: H H0; rewrite /poly1305_pre /poly1305_post /poly1305_ref => //= /> *.
+ congr.
+ by move/storeW128_inj_w: H1; rewrite W128.to_uint_eq !of_uintK !modz_mod /#.
 (* Last block processing *)
 (* One last synched iteration? *)
 case (to_uint inl %% 16 = 0).
-seq 1 1 : ((#{/~n{1}}{~i{1}}pre) /\ inlen0{2} = W64.zero); 
-   last by auto => />.
-case (to_uint inl = 0).
-while (#pre). 
-exfalso. 
-rewrite /poly1305_pre. 
-move => &1 &2 [/ # *].
-smt. 
-auto => />.  
-move => &1 &2 [/ # *].
-progress.
-smt. smt. smt.
-
-(* One last synched iteration! *)
-while (#{/~n{1}}{~i{1}}pre /\ n{1} = size m{1} /\
+ seq 1 1 : ((#{/~n{1}}{~i{1}}pre) /\ inlen0{2} = W64.zero); last by auto.
+ case (to_uint inl = 0).
+  while (#pre). 
+   exfalso; rewrite /poly1305_pre. 
+   by move => &1 &2 [/ # *] /#.
+  auto => /> &1 &2 [/ # *]; rewrite !uleE; progress; first 2 smt().
+  smt(@W64).
+ (* One last synched iteration! *)
+ while (#{/~n{1}}{~i{1}}pre /\ n{1} = size m{1} /\
            in_0{2} = inn + (of_int (i{1} * 16))%W64 /\
            to_uint inlen0{2} = to_uint inlen{2} - 16 * i{1} /\
            ((to_uint inlen0{2} = 16 /\ n{1} -1 <= i{1}) \/
            (to_uint inlen0{2} = 0 /\ i{1} = n{1}))).
-auto => />.
-move => &1 &2 [/ # *].
-progress.
-elim H4; last by smt.
-move => *.
-rewrite H0 /mkseq onth_nth_map; 
-    rewrite (nth_map witness);
-      first by rewrite size_map size_iota /max;smt.
-    rewrite (nth_map witness);
-      first by rewrite size_iota /max;smt.
+  wp; skip; rewrite !uleE /poly1305_pre; progress.
+  + elim: H4; last smt().
+    move=> [??]; congr; congr.
+    rewrite H0 /mkseq onth_nth_map (nth_map witness) /=.
+     by rewrite size_map size_iota /max /= smt(size_ge0).
+    rewrite (nth_map witness).
+     by rewrite size_iota /max /= smt(size_ge0).
     auto => />.
-    rewrite nth_iota. smt. 
-rewrite (_: 0 + i{1} < size m{1} - 1 = false); first by smt. 
-simplify. rewrite /load_block. 
-rewrite (_ : inlen{2} - (of_int (i{1} * 16))%W64 = W64.of_int 16). 
-move : H. rewrite H1. simplify. move => *.
-smt. smt. smt.  by smt. smt. smt. smt.
-
-skip.
-move => &1 &2 [/ # *].
-progress => //=.
-smt. smt. smt. smt. smt.
-
+    rewrite nth_iota /=; first smt(size_ge0). 
+    have ->/=: ! i{1} < size m{1} - 1 by smt().
+    smt(@W64).
+  + smt().
+  + by rewrite to_uintB ?uleE //= /#.
+  + by rewrite !to_uintB ?uleE //= /#.
+  + by rewrite uleE to_uintB ?uleE //= /#.
+  + by move: H7; rewrite uleE to_uintB ?uleE //= /#.
+ skip; move => &1 &2 [/ # *]; progress => //=; rewrite ?uleE /=; first 3 smt().
+  + by move: H21; rewrite uleE /#.
+  + smt(@W64).
 (* Ref executes loop one more time *)
 unroll {1} 1.
 rcondt {1} 1.
-move => &m.
-skip.
-smt.
-
+move => &m; skip; rewrite /poly1305_pre; progress.
+ move: H5; rewrite H H6 /=; smt(W64.to_uint_cmp).
 seq  3 1: (#{/~ ={h}}{~i{1}}pre /\
+             h{1} = (h{2} + oget (onth m{1} (i{1}-1))) * r{1} /\
+             i{1} = n{1} /\
+             to_uint inlen0{2} = to_uint inlen{2} - 16 * (i{1}-1) /\
+             in_0{2} = inn + (of_int (16 * (i{1}-1)))%W64).
+ seq 2 0 : (#{/~ ={h}}{~i{1}}pre /\
+              to_uint inlen0{2} = to_uint inlen{2} - 16 * (i{1}-1) /\
               h{1} = (h{2} + oget (onth m{1} (i{1}-1))) * r{1} /\
               i{1} = n{1} /\
-              to_uint inlen0{2} = to_uint inlen{2} - 16 * (i{1}-1) /\
-    in_0{2} = inn + (of_int (16 * (i{1}-1)))%W64).
-seq 2 0 : (#{/~ ={h}}{~i{1}}pre /\
-              to_uint inlen0{2} = to_uint inlen{2} - 16 * (i{1}-1) /\
-              h{1} = (h{2} + oget (onth m{1} (i{1}-1))) * r{1} /\
-              i{1} = n{1} /\
-in_0{2} = inn + (of_int (16 * (i{1}-1)))%W64).
-auto => />. 
-move => &1 &2 i_L [/ # *]. 
-smt.
-while (#pre ).
-auto => />. 
-skip.
-move => &1 &2 [/ # *]. 
-progress. smt. smt. smt. smt. smt. smt. smt. smt.
-auto => />. 
-move => &1 &2 i_L [/ # *]. 
-progress.
-rewrite {1} H. rewrite /mkseq onth_nth_map. 
-rewrite (nth_map witness None Some). 
-smt. 
-rewrite (nth_map witness witness) => //=. 
-smt. 
-rewrite (_: nth witness (iota_ 0 (size m{1})) (size m{1} - 1) < size m{1} - 1 = false). smt.
-simplify.
-rewrite nth_iota. smt. 
-rewrite (_: ((size m{1} - 1)) * 16 = 16 * (size m{1} - 1)). smt.
-have __: (inlen0{2} = inlen{2} - W64.of_int (16 * (size m{1} - 1))). 
-apply W64.word_modeqP. 
-rewrite to_uintB. smt. smt. smt. smt.
+              in_0{2} = inn + (of_int (16 * (i{1}-1)))%W64).
+  auto => /> &1 &2 i_L [/ # *]. 
+  move: H4; rewrite i_L H5 /=; smt(W64.to_uint_cmp).
+ while (#pre ); first by auto.
+ skip => &1 &2 [/ # *]; progress; first 7 smt().
+ by move: H17; rewrite uleE /= /#.
+auto => /> &1 &2 i_L [/ # *]; progress.
+ rewrite {1}H /mkseq onth_nth_map (nth_map witness None Some). 
+  move: H2; rewrite ultE size_map size_iota /max /=. 
+  smt(size_ge0 W64.to_uint_cmp).
+ rewrite (nth_map witness witness) => //=. 
+  move: H2; rewrite ultE size_iota /max /=.
+  smt(size_ge0 W64.to_uint_cmp).
+ rewrite (_:! nth witness (iota_ 0 (size m{1})) (size m{1} - 1) < size m{1}-1).  move: H2; rewrite ultE nth_iota i_L !H0 /=; smt(divz_ge0 W64.to_uint_cmp).
+ rewrite /= nth_iota.
+  rewrite i_L !H0 /=; smt(divz_ge0 W64.to_uint_cmp).
+ congr; congr; congr.
+  apply W64.word_modeqP; congr; congr.
+  rewrite to_uintB ?uleE //= of_uintK.
+   rewrite modz_small.
+    apply bound_abs; rewrite i_L H0 /=; split; first smt(W64.to_uint_cmp).
+    move => ?; rewrite -ltz_divRL //= ltz_divLR //=.
+    move: (W64.to_uint_cmp inlen{2}); smt().
+   smt(@W64).
+  rewrite modz_small. 
+   apply bound_abs; rewrite i_L H0 /=; split; first smt(W64.to_uint_cmp).
+   move => ?; rewrite -ltz_divRL //= ltz_divLR //=.
+   move: (W64.to_uint_cmp inlen{2}); smt().
+  smt().
+ smt().
+smt(@W64).
 qed.
 
 lemma corr mem rr ss mm outt inn inl kk :
@@ -364,19 +362,20 @@ lemma corr mem rr ss mm outt inn inl kk :
    Mspec.poly1305 : 
       Glob.mem = mem /\
       out = outt /\ in_0 = inn /\ inlen = inl /\ k = kk /\
-      poly1305_pre rr ss mm mem inn inl kk ==> 
-    poly1305_post mem Glob.mem outt rr ss mm] = 1%r.
+      poly1305_pre rr ss mm mem inn inl kk
+    ==> 
+      poly1305_post mem Glob.mem outt rr ss mm] = 1%r.
 proof.
 bypr => &m pxm.
-  rewrite -(_ :
-       Pr[Poly1305_RefWhile.poly1305(rr, ss, mm) @ &m :
-          res = poly1305_ref rr ss mm  ] = 1%r).
-by byphoare (_ :  m = mm /\ r = rr /\ s=ss ==> res = poly1305_ref rr ss mm) => //;
-apply: (ref_ok_ll mm rr ss).
-have ? : (Pr[Poly1305_RefWhile.poly1305(rr, ss, mm) @ &m : res = poly1305_ref rr ss mm] = 
-Pr[Mspec.poly1305(out{m}, in_0{m}, inlen{m}, k{m}) @ &m :
-   poly1305_post mem Glob.mem outt rr ss mm]); last by smt().
-byequiv => //=. proc*.
+rewrite -(_: Pr[Poly1305_RefWhile.poly1305(rr, ss, mm) @ &m :
+                   res = poly1305_ref rr ss mm  ] = 1%r).
+ byphoare (_: m = mm /\ r = rr /\ s=ss ==> res = poly1305_ref rr ss mm) => //.
+ by apply: (ref_ok_ll mm rr ss).
+have ? : (Pr[Poly1305_RefWhile.poly1305(rr, ss, mm) @ &m :
+                res = poly1305_ref rr ss mm] = 
+          Pr[Mspec.poly1305(out{m}, in_0{m}, inlen{m}, k{m}) @ &m :
+                poly1305_post mem Glob.mem outt rr ss mm]); last by smt().
+byequiv => //=; proc*.
 call (spec_eq mem rr ss mm outt inn inl kk).  
 by auto => />.
 qed.
