proof/crypto_onetimeauth/poly1305/asyncloop.ec
@@ -49,7 +49,7 @@ inlen02 < 128 => !(128 <= inlen1 /\ 128 <= inlen1 /% 64 * 64) =>
 lemma aux  a b n :
      a %% 4 = 0 => a < n =>
      n <= a + 4 => (n <= b \/ n <= b %/ 4 * 4 + 4) =>
-     (b = a \/ b+1 = a \/ b+2 = a \/ b+3 = a) => b = a by smt.
+     (b = a \/ b+1 = a \/ b+2 = a \/ b+3 = a) => b = a by smt().
 
 equiv asyncloop : M.f ~ M.g : ={arg} ==> ={res}.
 proof.
@@ -57,7 +57,7 @@ proc.
 splitwhile {1} 2 : (i %/ 4 * 4 + 4 < n).
 seq 1 1 : (#pre /\ (i{1} = i{2})); first by auto => />.
 seq 1 1 : #pre.
-async while
+ async while
   [ f (i%r), p (i{2})%r ]
   [ g (i%r), q (i{1})%r ]
     (inv1 (={i}))
@@ -67,45 +67,43 @@ async while
         (i{1} + 1 = i{2} /\ a{2} = (a{1} + 1)*b{1}) \/ 
         (i{1} + 2 = i{2} /\ a{2} = ((a{1} + 1)*b{1} + 1) * b{1})  \/ 
         (i{1} + 3 = i{2} /\ a{2} = (((a{1} + 1)*b{1} + 1) * b{1} + 1) * b{1})))).
-(* inv3 => c1 \/ c2 => inv1 => c1 /\ c2 /\ f p /\ g q *)
-rewrite /c1 /c2 /inv3 /inv1 /f /g;smt.
-(* inv3 => c1 \/ c2 => !inv1 => inv2 => c1 *)
-rewrite /c1 /c2 /inv3 /inv1 /inv2 /f /g;smt.
-(* inv3 => c1 \/ c2 => !inv1 => !inv2 => c2 *)
-rewrite /c1 /c2 /inv3 /inv1 /inv2 /f /g => /#.
-(* {inv3 /\ c1 /\ !inv1 /\ inv2} Body1 {inv3} *)
-rewrite /c1 /c2 /inv3 /inv1 /inv2 /f /g.
-by auto => />;smt.
-(* { inv3 /\ c2 /\ !inv1 /\ !inv2} Body2 {inv3} *)
-rewrite /c1 /c2 /inv3 /inv1 /inv2 /f /g.
-by auto => /#.
-(*
-forall v1 v2,
-{inv3 /\ (c1 \/ c2) /\ inv1 /\ v1_ = p /\ v2_ = q}
-    while (c1 /\ f v1) Body1 ~ while (c2 /\ g v2) Body2
-{inv3}
-*)
-move => *.
-while(i{2} <= n{1} /\ ={n,b} /\ (i{2} %% 4 = 0) /\ (n{2} <= i{2} + 4 => i{2} < n{2}) /\
+ - (* inv3 => c1 \/ c2 => inv1 => c1 /\ c2 /\ f p /\ g q *)
+   by rewrite /c1 /c2 /inv3 /inv1 /f /g /#.
+ - (* inv3 => c1 \/ c2 => !inv1 => inv2 => c1 *)
+   by rewrite /c1 /c2 /inv3 /inv1 /inv2 /f /g /#.
+ - (* inv3 => c1 \/ c2 => !inv1 => !inv2 => c2 *)
+   by rewrite /c1 /c2 /inv3 /inv1 /inv2 /f /g /#.
+ - (* {inv3 /\ c1 /\ !inv1 /\ inv2} Body1 {inv3} *)
+   rewrite /c1 /c2 /inv3 /inv1 /inv2 /f /g.
+   by auto => /> /#.
+ - (* { inv3 /\ c2 /\ !inv1 /\ !inv2} Body2 {inv3} *)
+   rewrite /c1 /c2 /inv3 /inv1 /inv2 /f /g.
+   by auto => /#.
+ - (* forall v1 v2,
+        {inv3 /\ (c1 \/ c2) /\ inv1 /\ v1_ = p /\ v2_ = q}
+          while (c1 /\ f v1) Body1 ~ while (c2 /\ g v2) Body2
+        {inv3}
+   *)
+   move => *.
+   while(i{2} <= n{1} /\ ={n,b} /\ (i{2} %% 4 = 0) /\ (n{2} <= i{2} + 4 => i{2} < n{2}) /\
       ((i{1} = i{2} /\ v1_ = i{2}%r /\ v2_ = i{1}%r /\ ={a}) \/ 
        (i{1} + 3 = i{2} /\ a{2} = (((a{1} + 1)*b{1} + 1) * b{1} + 1) * b{1} 
             /\ v1_ = i{2}%r - 4%r /\ v2_ = i{1}%r - 1%r))).
-wp;skip;progress;
-[smt() | smt | smt |
-case (i{1} = i{2} /\ v1_ = i{2}%r /\ v2_ = i{1}%r /\ a{1} = a{2}) => /# | 
-       smt() | smt() | smt() | smt() | smt() ].
-by auto => />;smt.
-(* inv3 ==> islossless while(c1 /\ !inv1 /\ inv2) Body1 *)
-while (true) (n-i).
-by auto => /#.
-by auto => /#.
-(* inv3 ==> islossless while(c1 /\ !inv1 /\ !inv2) Body2 *)
-while (true) (n-i).
-by auto => /#.
-by auto => /#.
-(* !c1 => !c2 => inv3 => #post *)
-skip;progress.
-   have ? : (i_L = i_R). apply : (aux i_R i_L n{2});smt(). smt().
-   apply : (aux i_R i_L n{2});smt(). 
+    wp;skip;progress; smt().
+   by auto => /> *; progress; smt().
+ - (* inv3 ==> islossless while(c1 /\ !inv1 /\ inv2) Body1 *)
+   while (true) (n-i).
+    by auto => /#.
+   by auto => /#.
+ - (* inv3 ==> islossless while(c1 /\ !inv1 /\ !inv2) Body2 *)
+   while (true) (n-i).
+    by auto => /#.
+   by auto => /#.
+ - (* !c1 => !c2 => inv3 => #post *)
+   skip;progress.
+    have ? : (i_L = i_R).
+     apply : (aux i_R i_L n{2}); smt().
+    smt().
+   by apply : (aux i_R i_L n{2}); smt(). 
 by sim />.
 qed.
